Playing around with binary search trees

teaching/taltech2018/sol/BinarySearchTree.fst
@@ -4,15 +4,37 @@ abstract type btree =
   | Leaf : btree
   | Node : btree -> nat -> btree -> btree
 
+let rec exists_in (n:nat) (t:btree) : GTot bool =
+  match t with 
+  | Leaf -> false
+  | Node t1 m t2 -> 
+      if n = m then true else 
+      if n < m then n `exists_in` t1 
+               else n `exists_in` t2
+
+let empty () : GTot btree = Leaf
+
+let rec insert (t:btree) (n:nat) : GTot btree =
+  match t with 
+  | Leaf -> Node Leaf n Leaf
+  | Node t1 m t2 -> 
+      if n = m then Node t1 m t2 else
+      if n < m then Node (insert t1 n) m t2
+               else Node t1 m (insert t2 n)
+
 let rec is_sorted_left (t:btree) (n:nat) : GTot bool = 
   match t with
   | Leaf -> true
-  | Node t1 m t2 -> t1 `is_sorted_left` m && m < n && t2 `is_sorted_right` m
+  | Node t1 m t2 -> t1 `is_sorted_left` m && 
+                    m < n && 
+                    t2 `is_sorted_right` m
 
 and is_sorted_right (t:btree) (n:nat) : GTot bool = 
   match t with
   | Leaf -> true
-  | Node t1 m t2 -> t1 `is_sorted_left` m && m > n && t2 `is_sorted_right` m
+  | Node t1 m t2 -> t1 `is_sorted_left` m && 
+                    m > n && 
+                    t2 `is_sorted_right` m
 
 let rec is_sorted (t:btree) : GTot bool =
   match t with
@@ -22,6 +44,34 @@ let rec is_sorted (t:btree) : GTot bool =
 abstract type stree = 
   t:btree{is_sorted t}
 
+let lemma_empty_is_sorted () : Lemma (is_sorted (empty ())) = 
+  ()
+
+let rec lemma_insert_is_sorted (t:stree) (n:nat) : Lemma (is_sorted (insert t n)) = 
+  match t with
+  | Leaf -> ()
+  | Node t1 m t2 -> 
+      if n = m then () else
+      if n < m then lemma_insert_is_sorted t1 n
+               else lemma_insert_is_sorted t2 n
+
+let rec lemma_exists_insert_equal (t:stree) (n:nat) : Lemma (requires (n `exists_in` t))
+                                                            (ensures  (insert t n = t)) = 
+  match t with
+  | Node t1 m t2 -> 
+      if n = m then () else 
+      if n < m then lemma_exists_insert_equal t1 n
+               else lemma_exists_insert_equal t2 n
+
+let rec lemma_insert_exists (t:stree) (n:nat) : Lemma (n `exists_in` (insert t n)) =
+  match t with
+  | Leaf -> ()
+  | Node t1 m t2 -> 
+      if n = m then () else
+      if n < m then lemma_insert_exists t1 n
+               else lemma_insert_exists t2 n
+
+(*
 let rec lemma_sorted_left_is_sorted (t:btree) (n:nat) : Lemma (requires (is_sorted_left t n))
                                                               (ensures  (is_sorted t)) 
                                                               [SMTPat (is_sorted_left t n)] =
@@ -37,11 +87,4 @@ and lemma_sorted_right_is_sorted (t:btree) (n:nat) : Lemma (requires (is_sorted_
   | Leaf -> ()
   | Node t1 m t2 -> lemma_sorted_left_is_sorted t1 m;
                     lemma_sorted_right_is_sorted t2 m
-
-let rec search (t:stree) (n:nat) : GTot bool =
-  match t with 
-  | Leaf -> false
-  | Node t1 m t2 -> 
-      if n = m then true else 
-      if n < m then search t1 n else
-                    search t2 n
+*)
